\documentclass{article}

\usepackage{fontspec}
\setmainfont{Times New Roman} % police d'écriture

\usepackage{tikz}
\usepackage{amsmath}

\usepackage[french]{babel}

\usepackage[a4paper,left=0.2cm,right=0.2cm,top=0.2cm,bottom=0.2cm]{geometry}

% Document
\begin{document}

    \begin{tikzpicture}
        \node (x) at (3.2,0) {$\overrightarrow{y_{0}}$};
        \node (y) at (0,3.2) {$\overrightarrow{z_{0}}$};
        \node (z) at (-0.2,-0.5) {$\overrightarrow{x_{0}} = \overrightarrow{x_{1}}$};

        \node (xone) at (3.2,1.1) {$\overrightarrow{y_{1}}$};
        \node (yone) at (-1.1,3.2) {$\overrightarrow{z_{1}}$};


        \draw[thick, ->] (3,0.1) arc (0:15:3);
        \node (alphab) at (3.2,0.5) {$\alpha$};
        \draw[thick, ->, rotate=90] (3,0.1) arc (0:16:3);
        \node (alphat) at (-0.5,3.2) {$\alpha$};

        \draw[->,line width=0.03cm] (0,0) to (3,0);
        \draw[->,line width=0.03cm] (0,0) to (0,3);

        \draw[->,line width=0.03cm] (0,0) to (2.85,0.95);
        \draw[->,line width=0.03cm] (0,0) to (-0.95,2.85);

        \node[circle,fill,color=white] (a) at (0,0) {};

        \node[circle,draw,line width=1pt] (a) at (0,0) {};
        \node[circle,fill,inner sep=1pt] (b) at (0, 0) {};
    \end{tikzpicture}
    \begin{tikzpicture}
        \node (x) at (3.2,0) {$\overrightarrow{y_{0}}$};
        \node (y) at (0,3.2) {$\overrightarrow{z_{0}}$};
        \node (z) at (-0.2,-0.5) {$\overrightarrow{x_{0}} = \overrightarrow{x_{2}}$};

        \node (xone) at (3.2,1.1) {$\overrightarrow{y_{2}}$};
        \node (yone) at (-1.1,3.2) {$\overrightarrow{z_{2}}$};


        \draw[thick, ->] (3,0.1) arc (0:15:3);
        \node (alphab) at (3.2,0.5) {$\theta$};
        \draw[thick, ->, rotate=90] (3,0.1) arc (0:16:3);
        \node (alphat) at (-0.5,3.2) {$\theta$};

        \draw[->,line width=0.03cm] (0,0) to (3,0);
        \draw[->,line width=0.03cm] (0,0) to (0,3);

        \draw[->,line width=0.03cm] (0,0) to (2.85,0.95);
        \draw[->,line width=0.03cm] (0,0) to (-0.95,2.85);

        \node[circle,fill,color=white] (a) at (0,0) {};

        \node[circle,draw,line width=1pt] (a) at (0,0) {};
        \node[circle,fill,inner sep=1pt] (b) at (0, 0) {};
    \end{tikzpicture}

    $\begin{bmatrix}A_{1} & 0 & 0\\\\0 & B_{1} & 0\\\\0 & 0 & B_{1}\end{bmatrix}$

    $\begin{bmatrix}A_{2} & 0 & - E_{2}\\\\0 & B_{2} & 0\\\\- E_{2} & 0 & C_{2}\end{bmatrix}$

    $\begin{bmatrix}A_{3} & 0 & 0\\\\0 & B_{3} & 0\\\\0 & 0 & B_{3}\end{bmatrix}$

    $\lambda \times \dot{\theta} \cdot \overrightarrow{y_{2}}$

    $( - E_{2} \times \dot{\theta} \cdot \overrightarrow{x_{2}} + 0 \cdot \overrightarrow{y_{2}} + C_{2} \times \dot{\theta} \cdot \overrightarrow{z_{2}} - ((a \cdot \overrightarrow{z_{0}} + \lambda \cdot \overrightarrow{x_{2}}) \land M_2 \cdot ((a \cdot \overrightarrow{z_{0}} + \lambda \cdot \overrightarrow{x_{2}}) \land \dot{\theta} \cdot \overrightarrow{z_{2}})))$

    $( - E_{2} \times \dot{\theta} \cdot \overrightarrow{x_{2}} + C_{2} \times \dot{\theta} \cdot \overrightarrow{z_{2}} - a \times M_2 \times \lambda \times \dot{\theta} \cdot \overrightarrow{x_{2}} + \lambda \times M_2 \times \lambda \times \dot{\theta} \cdot \overrightarrow{z_{2}})$

    \vspace{5em}

    $-\left.\dfrac{d ((a \cdot \overrightarrow{z_{0}} + \lambda \cdot \overrightarrow{x_{2}}) \land \dot{\theta} \cdot \overrightarrow{z_{2}})}{dt}\right|_{R_{0}}$

    $( - E_{2} \times \ddot{\theta} \cdot \overrightarrow{x_{2}} +  - E_{2} \times \dot{\theta} \cdot (\dot{\theta} \cdot \overrightarrow{z_{2}} \land \overrightarrow{x_{2}}) + 0 \cdot \overrightarrow{y_{2}} + 0 \cdot (\dot{\theta} \cdot \overrightarrow{z_{2}} \land \overrightarrow{y_{2}}) + C_{2} \times \ddot{\theta} \cdot \overrightarrow{z_{2}} + C_{2} \times \dot{\theta} \cdot (\dot{\theta} \cdot \overrightarrow{z_{2}} \land \overrightarrow{z_{2}}) - ((a \cdot \overrightarrow{z_{0}} + \lambda \cdot \overrightarrow{x_{2}}) \land M_2 \cdot \left.\dfrac{d ((a \cdot \overrightarrow{z_{0}} + \lambda \cdot \overrightarrow{x_{2}}) \land \dot{\theta} \cdot \overrightarrow{z_{2}})}{dt}\right|_{R_{0}}))$

    $( - E_{2} \times \ddot{\theta} \cdot \overrightarrow{x_{2}} - E_{2} \times \dot{\theta} \times \dot{\theta} \cdot \overrightarrow{y_{2}} + C_{2} \times \ddot{\theta} \cdot \overrightarrow{z_{2}} - a \times M_2 \cdot ((\overrightarrow{z_{0}} \land \lambda \times \dot{\theta} \times \dot{\theta} \cdot \overrightarrow{x_{2}}) + (\overrightarrow{z_{0}} \land (a \cdot 0 + \lambda \cdot  - \ddot{\theta} \cdot \overrightarrow{y_{2}}))) - \lambda \times M_2 \cdot ((\overrightarrow{x_{2}} \land \lambda \times \dot{\theta} \times \dot{\theta} \cdot \overrightarrow{x_{2}}) + (\overrightarrow{x_{2}} \land (a \cdot 0 + \lambda \cdot  - \ddot{\theta} \cdot \overrightarrow{y_{2}}))))$

    $( - E_{2} \times \ddot{\theta} \cdot \overrightarrow{x_{2}} - E_{2} \times \dot{\theta} \times \dot{\theta} \cdot \overrightarrow{y_{2}} + C_{2} \times \ddot{\theta} \cdot \overrightarrow{z_{2}} - a \times M_2 \cdot (\lambda \times \dot{\theta} \times \dot{\theta} \cdot \overrightarrow{y_{2}} + \lambda \times \ddot{\theta} \cdot \overrightarrow{x_{2}}) - \lambda \times M_2 \cdot  - \lambda \times \ddot{\theta} \cdot \overrightarrow{z_{2}})$

    $( - E_{2} \times \ddot{\theta} \cdot \overrightarrow{x_{2}} - E_{2} \times \dot{\theta} \times \dot{\theta} \cdot \overrightarrow{y_{2}} + C_{2} \times \ddot{\theta} \cdot \overrightarrow{z_{2}} - a \times M_2 \cdot (\lambda \times \dot{\theta} \times \dot{\theta} \cdot \overrightarrow{y_{2}} + \lambda \times \ddot{\theta} \cdot \overrightarrow{x_{2}}) + \lambda \times M_2 \times \lambda \times \ddot{\theta} \cdot \overrightarrow{z_{2}})$

    $( - E_{2} \times \ddot{\theta} \cdot \overrightarrow{x_{2}} - E_{2} \times \dot{\theta} \times \dot{\theta} \cdot \overrightarrow{y_{2}} + C_{2} \times \ddot{\theta} \cdot \overrightarrow{z_{2}} - a \times M_2 \cdot (\lambda \times \dot{\theta} \times \dot{\theta} \cdot \overrightarrow{y_{2}} + \lambda \times \ddot{\theta} \cdot \overrightarrow{x_{2}}) + \lambda \times M_2 \times \lambda \times \ddot{\theta} \cdot \overrightarrow{z_{2}})$

    \vspace{5em}

    $( - (E_{2} \times \ddot{\theta} \cdot \overrightarrow{x_{2}} + E_{2} \times \dot{\theta} \cdot (\dot{\theta} \cdot \overrightarrow{z_{2}} \land \overrightarrow{x_{2}})) + (C_{2} \times \ddot{\theta} \cdot \overrightarrow{z_{2}} + C_{2} \times \dot{\theta} \cdot (\dot{\theta} \cdot \overrightarrow{z_{2}} \land \overrightarrow{z_{2}})) - ((a \cdot \overrightarrow{z_{0}} + \lambda \cdot \overrightarrow{x_{2}}) \land M_2 \cdot \left.\dfrac{d ((a \cdot \overrightarrow{z_{0}} + \lambda \cdot \overrightarrow{x_{2}}) \land \dot{\theta} \cdot \overrightarrow{z_{2}})}{dt}\right|_{R_{0}}))$

    $( - (E_{2} \times \ddot{\theta} \cdot \overrightarrow{x_{2}} + E_{2} \times \dot{\theta} \times \dot{\theta} \cdot \overrightarrow{y_{2}}) + (C_{2} \times \ddot{\theta} \cdot \overrightarrow{z_{2}} + \vec{0}) - (a \times M_2 \cdot ((\overrightarrow{z_{0}} \land \lambda \times \dot{\theta} \times \dot{\theta} \cdot \overrightarrow{x_{2}}) + (\overrightarrow{z_{0}} \land (a \cdot (\vec{0} + \dot{\theta} \cdot (\overrightarrow{z_{0}} \land \vec{0})) + \lambda \cdot ( - \ddot{\theta} \cdot \overrightarrow{y_{2}} + \dot{\theta} \cdot (\overrightarrow{x_{2}} \land \vec{0}))))) + \lambda \times M_2 \cdot ((\overrightarrow{x_{2}} \land \lambda \times \dot{\theta} \times \dot{\theta} \cdot \overrightarrow{x_{2}}) + (\overrightarrow{x_{2}} \land (a \cdot (\vec{0} + \dot{\theta} \cdot (\overrightarrow{z_{0}} \land \vec{0})) + \lambda \cdot ( - \ddot{\theta} \cdot \overrightarrow{y_{2}} + \dot{\theta} \cdot (\overrightarrow{x_{2}} \land \vec{0})))))))$

    $( - (E_{2} \times \ddot{\theta} \cdot \overrightarrow{x_{2}} + E_{2} \times \dot{\theta} \times \dot{\theta} \cdot \overrightarrow{y_{2}}) + (C_{2} \times \ddot{\theta} \cdot \overrightarrow{z_{2}} + \vec{0}) - (a \times M_2 \cdot (\lambda \times \dot{\theta} \times \dot{\theta} \cdot \overrightarrow{y_{2}} + (\vec{0} + \lambda \times \ddot{\theta} \cdot \overrightarrow{x_{2}})) + \lambda \times M_2 \cdot (\vec{0} + (\vec{0} - \lambda \times \ddot{\theta} \cdot \overrightarrow{z_{2}}))))$

    $( - (E_{2} \times \ddot{\theta} \cdot \overrightarrow{x_{2}} + E_{2} \times \dot{\theta} \times \dot{\theta} \cdot \overrightarrow{y_{2}}) + (C_{2} \times \ddot{\theta} \cdot \overrightarrow{z_{2}} + \vec{0}) - (a \times M_2 \cdot (\lambda \times \dot{\theta} \times \dot{\theta} \cdot \overrightarrow{y_{2}} + (\vec{0} + \lambda \times \ddot{\theta} \cdot \overrightarrow{x_{2}})) + \lambda \times M_2 \cdot (\vec{0} + (\vec{0} - \lambda \times \ddot{\theta} \cdot \overrightarrow{z_{2}}))))$

    $( - (E_{2} \times \ddot{\theta} \cdot \overrightarrow{x_{2}} + E_{2} \times \dot{\theta} \times \dot{\theta} \cdot \overrightarrow{y_{2}}) + (C_{2} \times \ddot{\theta} \cdot \overrightarrow{z_{2}} + \vec{0}) - (a \times M_2 \cdot (\lambda \times \dot{\theta} \times \dot{\theta} \cdot \overrightarrow{y_{2}} + (\vec{0} + \lambda \times \ddot{\theta} \cdot \overrightarrow{x_{2}})) + \lambda \times M_2 \cdot (\vec{0} + (\vec{0} - \lambda \times \ddot{\theta} \cdot \overrightarrow{z_{2}}))))$

    \vspace{5em}

    $( - E_{2} \times \ddot{\theta} \cdot \overrightarrow{x_{2}} - E_{2} \times \dot{\theta} \cdot (\dot{\theta} \cdot \overrightarrow{z_{2}} \land \overrightarrow{x_{2}}) + C_{2} \times \ddot{\theta} \cdot \overrightarrow{z_{2}} + C_{2} \times \dot{\theta} \cdot (\dot{\theta} \cdot \overrightarrow{z_{2}} \land \overrightarrow{z_{2}}) - ((a \cdot \overrightarrow{z_{0}} + \lambda \cdot \overrightarrow{x_{2}}) \land M_2 \cdot \left.\dfrac{d ((a \cdot \overrightarrow{z_{0}} + \lambda \cdot \overrightarrow{x_{2}}) \land \dot{\theta} \cdot \overrightarrow{z_{2}})}{dt}\right|_{R_{0}}))$

    $( - E_{2} \times \ddot{\theta} \cdot \overrightarrow{x_{2}} - E_{2} \times \dot{\theta} \times \dot{\theta} \cdot \overrightarrow{y_{2}} + C_{2} \times \ddot{\theta} \cdot \overrightarrow{z_{2}} + \vec{0} - (a \times M_2 \cdot ((\overrightarrow{z_{0}} \land \lambda \times \dot{\theta} \times \dot{\theta} \cdot \overrightarrow{x_{2}}) + (\overrightarrow{z_{0}} \land (a \cdot (\vec{0} + \dot{\theta} \cdot (\overrightarrow{z_{0}} \land \vec{0})) + \lambda \cdot ( - \ddot{\theta} \cdot \overrightarrow{y_{2}} + \dot{\theta} \cdot (\overrightarrow{x_{2}} \land \vec{0}))))) + \lambda \times M_2 \cdot ((\overrightarrow{x_{2}} \land \lambda \times \dot{\theta} \times \dot{\theta} \cdot \overrightarrow{x_{2}}) + (\overrightarrow{x_{2}} \land (a \cdot (\vec{0} + \dot{\theta} \cdot (\overrightarrow{z_{0}} \land \vec{0})) + \lambda \cdot ( - \ddot{\theta} \cdot \overrightarrow{y_{2}} + \dot{\theta} \cdot (\overrightarrow{x_{2}} \land \vec{0})))))))$

    $( - E_{2} \times \ddot{\theta} \cdot \overrightarrow{x_{2}} - E_{2} \times \dot{\theta} \times \dot{\theta} \cdot \overrightarrow{y_{2}} + C_{2} \times \ddot{\theta} \cdot \overrightarrow{z_{2}} + \vec{0} - (a \times M_2 \cdot (\lambda \times \dot{\theta} \times \dot{\theta} \cdot \overrightarrow{y_{2}} + (\vec{0} + \lambda \times \ddot{\theta} \cdot \overrightarrow{x_{2}})) + \lambda \times M_2 \cdot (\vec{0} + (\vec{0} - \lambda \times \ddot{\theta} \cdot \overrightarrow{z_{2}}))))$

    $( - E_{2} \times \ddot{\theta} \cdot \overrightarrow{x_{2}} - E_{2} \times \dot{\theta} \times \dot{\theta} \cdot \overrightarrow{y_{2}} + C_{2} \times \ddot{\theta} \cdot \overrightarrow{z_{2}} + \vec{0} - (a \times M_2 \cdot (\lambda \times \dot{\theta} \times \dot{\theta} \cdot \overrightarrow{y_{2}} + (\vec{0} + \lambda \times \ddot{\theta} \cdot \overrightarrow{x_{2}})) + \lambda \times M_2 \cdot (\vec{0} + (\vec{0} - \lambda \times \ddot{\theta} \cdot \overrightarrow{z_{2}}))))$

    $( - E_{2} \times \ddot{\theta} \cdot \overrightarrow{x_{2}} - E_{2} \times \dot{\theta} \times \dot{\theta} \cdot \overrightarrow{y_{2}} + C_{2} \times \ddot{\theta} \cdot \overrightarrow{z_{2}} + \vec{0} - (a \times M_2 \cdot (\lambda \times \dot{\theta} \times \dot{\theta} \cdot \overrightarrow{y_{2}} + (\vec{0} + \lambda \times \ddot{\theta} \cdot \overrightarrow{x_{2}})) + \lambda \times M_2 \cdot (\vec{0} + (\vec{0} - \lambda \times \ddot{\theta} \cdot \overrightarrow{z_{2}}))))$

    \vspace{5em}

    $( - E_{2} \times \ddot{\theta} \cdot \overrightarrow{x_{2}} - E_{2} \times \dot{\theta} \cdot (\dot{\theta} \cdot \overrightarrow{z_{2}} \land \overrightarrow{x_{2}}) + C_{2} \times \ddot{\theta} \cdot \overrightarrow{z_{2}} + C_{2} \times \dot{\theta} \cdot (\dot{\theta} \cdot \overrightarrow{z_{2}} \land \overrightarrow{z_{2}}) - ((a \cdot \overrightarrow{z_{0}} + \lambda \cdot \overrightarrow{x_{2}}) \land M_2 \cdot \left.\dfrac{d ((a \cdot \overrightarrow{z_{0}} + \lambda \cdot \overrightarrow{x_{2}}) \land \dot{\theta} \cdot \overrightarrow{z_{2}})}{dt}\right|_{R_{0}}))$

    $( - E_{2} \times \ddot{\theta} \cdot \overrightarrow{x_{2}} - E_{2} \times \dot{\theta} \times \dot{\theta} \cdot \overrightarrow{y_{2}} + C_{2} \times \ddot{\theta} \cdot \overrightarrow{z_{2}} + \vec{0} - (a \times M_2 \cdot ((\overrightarrow{z_{0}} \land \lambda \times \dot{\theta} \times \dot{\theta} \cdot \overrightarrow{x_{2}}) + (\overrightarrow{z_{0}} \land (a \cdot (\vec{0} + \dot{\theta} \cdot (\overrightarrow{z_{0}} \land \vec{0})) + \lambda \cdot ( - \ddot{\theta} \cdot \overrightarrow{y_{2}} + \dot{\theta} \cdot (\overrightarrow{x_{2}} \land \vec{0}))))) + \lambda \times M_2 \cdot ((\overrightarrow{x_{2}} \land \lambda \times \dot{\theta} \times \dot{\theta} \cdot \overrightarrow{x_{2}}) + (\overrightarrow{x_{2}} \land (a \cdot (\vec{0} + \dot{\theta} \cdot (\overrightarrow{z_{0}} \land \vec{0})) + \lambda \cdot ( - \ddot{\theta} \cdot \overrightarrow{y_{2}} + \dot{\theta} \cdot (\overrightarrow{x_{2}} \land \vec{0})))))))$

    $( - E_{2} \times \ddot{\theta} \cdot \overrightarrow{x_{2}} - E_{2} \times \dot{\theta} \times \dot{\theta} \cdot \overrightarrow{y_{2}} + C_{2} \times \ddot{\theta} \cdot \overrightarrow{z_{2}} + \vec{0} - (a \times M_2 \cdot (\lambda \times \dot{\theta} \times \dot{\theta} \cdot \overrightarrow{y_{2}} + (\vec{0} + \lambda \times \ddot{\theta} \cdot \overrightarrow{x_{2}})) + \lambda \times M_2 \cdot (\vec{0} + (\vec{0} - \lambda \times \ddot{\theta} \cdot \overrightarrow{z_{2}}))))$

    $( - E_{2} \times \ddot{\theta} \cdot \overrightarrow{x_{2}} - E_{2} \times \dot{\theta} \times \dot{\theta} \cdot \overrightarrow{y_{2}} + C_{2} \times \ddot{\theta} \cdot \overrightarrow{z_{2}} + \vec{0} - (a \times M_2 \cdot (\lambda \times \dot{\theta} \times \dot{\theta} \cdot \overrightarrow{y_{2}} + (\vec{0} + \lambda \times \ddot{\theta} \cdot \overrightarrow{x_{2}})) + \lambda \times M_2 \cdot (\vec{0} + (\vec{0} - \lambda \times \ddot{\theta} \cdot \overrightarrow{z_{2}}))))$

    $( - E_{2} \times \ddot{\theta} \cdot \overrightarrow{x_{2}} - E_{2} \times \dot{\theta} \times \dot{\theta} \cdot \overrightarrow{y_{2}} + C_{2} \times \ddot{\theta} \cdot \overrightarrow{z_{2}} + \vec{0} - (a \times M_2 \cdot (\lambda \times \dot{\theta} \times \dot{\theta} \cdot \overrightarrow{y_{2}} + (\vec{0} + \lambda \times \ddot{\theta} \cdot \overrightarrow{x_{2}})) + \lambda \times M_2 \cdot (\vec{0} + (\vec{0} - \lambda \times \ddot{\theta} \cdot \overrightarrow{z_{2}}))))$

    \vspace{5em}

    $( - E_{2} \times \ddot{\theta} \cdot \overrightarrow{x_{2}} - E_{2} \times \dot{\theta} \cdot (\dot{\theta} \cdot \overrightarrow{z_{2}} \land \overrightarrow{x_{2}}) + C_{2} \times \ddot{\theta} \cdot \overrightarrow{z_{2}} + C_{2} \times \dot{\theta} \cdot (\dot{\theta} \cdot \overrightarrow{z_{2}} \land \overrightarrow{z_{2}}) - ((a \cdot \overrightarrow{z_{0}} + \lambda \cdot \overrightarrow{x_{2}}) \land M_2 \cdot \left.\dfrac{d ((a \cdot \overrightarrow{z_{0}} + \lambda \cdot \overrightarrow{x_{2}}) \land \dot{\theta} \cdot \overrightarrow{z_{2}})}{dt}\right|_{R_{0}}))$

    $( - E_{2} \times \ddot{\theta} \cdot \overrightarrow{x_{2}} - E_{2} \times \dot{\theta} \times \dot{\theta} \cdot \overrightarrow{y_{2}} + C_{2} \times \ddot{\theta} \cdot \overrightarrow{z_{2}} - a \times M_2 \cdot ((\overrightarrow{z_{0}} \land \lambda \times \dot{\theta} \times \dot{\theta} \cdot \overrightarrow{x_{2}}) - (\overrightarrow{z_{0}} \land \lambda \times \ddot{\theta} \cdot \overrightarrow{y_{2}})) - \lambda \times M_2 \cdot ((\overrightarrow{x_{2}} \land \lambda \times \dot{\theta} \times \dot{\theta} \cdot \overrightarrow{x_{2}}) - (\overrightarrow{x_{2}} \land \lambda \times \ddot{\theta} \cdot \overrightarrow{y_{2}})))$

    $( - E_{2} \times \ddot{\theta} \cdot \overrightarrow{x_{2}} - E_{2} \times \dot{\theta} \times \dot{\theta} \cdot \overrightarrow{y_{2}} + C_{2} \times \ddot{\theta} \cdot \overrightarrow{z_{2}} - a \times M_2 \cdot (\lambda \times \dot{\theta} \times \dot{\theta} \cdot \overrightarrow{y_{2}} + \lambda \times \ddot{\theta} \cdot \overrightarrow{x_{2}}) + \lambda \times M_2 \times \lambda \times \ddot{\theta} \cdot \overrightarrow{z_{2}})$

    $( - E_{2} \times \ddot{\theta} \cdot \overrightarrow{x_{2}} - E_{2} \times \dot{\theta} \times \dot{\theta} \cdot \overrightarrow{y_{2}} + C_{2} \times \ddot{\theta} \cdot \overrightarrow{z_{2}} - a \times M_2 \cdot (\lambda \times \dot{\theta} \times \dot{\theta} \cdot \overrightarrow{y_{2}} + \lambda \times \ddot{\theta} \cdot \overrightarrow{x_{2}}) + \lambda \times M_2 \times \lambda \times \ddot{\theta} \cdot \overrightarrow{z_{2}})$

    $( - E_{2} \times \ddot{\theta} \cdot \overrightarrow{x_{2}} - E_{2} \times \dot{\theta} \times \dot{\theta} \cdot \overrightarrow{y_{2}} + C_{2} \times \ddot{\theta} \cdot \overrightarrow{z_{2}} - a \times M_2 \cdot (\lambda \times \dot{\theta} \times \dot{\theta} \cdot \overrightarrow{y_{2}} + \lambda \times \ddot{\theta} \cdot \overrightarrow{x_{2}}) + \lambda \times M_2 \times \lambda \times \ddot{\theta} \cdot \overrightarrow{z_{2}})$

    \vspace{5em}

    \begin{align*}
        \overrightarrow{\delta_{O \in 2/0}}&=( - E_{2} \times \ddot{\theta} \cdot \overrightarrow{x_{2}} - E_{2} \times \dot{\theta} \cdot (\dot{\theta} \cdot \overrightarrow{z_{2}} \land \overrightarrow{x_{2}}) + C_{2} \times \ddot{\theta} \cdot \overrightarrow{z_{2}} + C_{2} \times \dot{\theta} \cdot (\dot{\theta} \cdot \overrightarrow{z_{2}} \land \overrightarrow{z_{2}}) - ((a \cdot \overrightarrow{z_{0}} + \lambda \cdot \overrightarrow{x_{2}}) \land M_2 \cdot \left.\dfrac{d ((a \cdot \overrightarrow{z_{0}} + \lambda \cdot \overrightarrow{x_{2}}) \land \dot{\theta} \cdot \overrightarrow{z_{2}})}{dt}\right|_{R_{0}}))\\
        &=( - E_{2} \times \ddot{\theta} \cdot \overrightarrow{x_{2}} - E_{2} \times \dot{\theta} \times \dot{\theta} \cdot \overrightarrow{y_{2}} + C_{2} \times \ddot{\theta} \cdot \overrightarrow{z_{2}} - a \times M_2 \cdot ((\overrightarrow{z_{0}} \land \lambda \times \dot{\theta} \times \dot{\theta} \cdot \overrightarrow{x_{2}}) - (\overrightarrow{z_{0}} \land \lambda \times \ddot{\theta} \cdot \overrightarrow{y_{2}})) - \lambda \times M_2 \cdot ((\overrightarrow{x_{2}} \land \lambda \times \dot{\theta} \times \dot{\theta} \cdot \overrightarrow{x_{2}}) - (\overrightarrow{x_{2}} \land \lambda \times \ddot{\theta} \cdot \overrightarrow{y_{2}})))\\
        &=( - E_{2} \times \ddot{\theta} \cdot \overrightarrow{x_{2}} - E_{2} \times \dot{\theta} \times \dot{\theta} \cdot \overrightarrow{y_{2}} + C_{2} \times \ddot{\theta} \cdot \overrightarrow{z_{2}} - a \times M_2 \cdot (\lambda \times \dot{\theta} \times \dot{\theta} \cdot \overrightarrow{y_{2}} + \lambda \times \ddot{\theta} \cdot \overrightarrow{x_{2}}) + \lambda \times M_2 \times \lambda \times \ddot{\theta} \cdot \overrightarrow{z_{2}})\\
    \end{align*}

    \newpage

    \begin{tabular}{cccc}
        \begin{tikzpicture}
            \node (x) at (3.2,0) {$\overrightarrow{x_{0}}$};
            \node (y) at (0,3.2) {$\overrightarrow{y_{0}}$};
            \node (z) at (-0.2,-0.5) {$\overrightarrow{z_{0}} = \overrightarrow{z_{1}}$};

            \node (xone) at (3.2,1.1) {$\overrightarrow{x_{1}}$};
            \node (yone) at (-1.1,3.2) {$\overrightarrow{y_{1}}$};


            \draw[thick, ->] (3,0.1) arc (0:15:3);
            \node (alphab) at (3.2,0.5) {$\alpha$};
            \draw[thick, ->, rotate=90] (3,0.1) arc (0:16:3);
            \node (alphat) at (-0.5,3.2) {$\alpha$};

            \draw[->,line width=0.03cm] (0,0) to (3,0);
            \draw[->,line width=0.03cm] (0,0) to (0,3);

            \draw[->,line width=0.03cm] (0,0) to (2.85,0.95);
            \draw[->,line width=0.03cm] (0,0) to (-0.95,2.85);

            \node[circle,fill,color=white] (a) at (0,0) {};

            \node[circle,draw,line width=1pt] (a) at (0,0) {};
            \node[circle,fill,inner sep=1pt] (b) at (0, 0) {};
        \end{tikzpicture} & \begin{tikzpicture}
                                \node (x) at (3.2,0) {$\overrightarrow{x_{0}}$};
                                \node (y) at (0,3.2) {$\overrightarrow{y_{0}}$};
                                \node (z) at (-0.2,-0.5) {$\overrightarrow{z_{0}} = \overrightarrow{z_{2}}$};

                                \node (xone) at (3.2,1.1) {$\overrightarrow{x_{2}}$};
                                \node (yone) at (-1.1,3.2) {$\overrightarrow{y_{2}}$};


                                \draw[thick, ->] (3,0.1) arc (0:15:3);
                                \node (alphab) at (3.2,0.5) {$\theta$};
                                \draw[thick, ->, rotate=90] (3,0.1) arc (0:16:3);
                                \node (alphat) at (-0.5,3.2) {$\theta$};

                                \draw[->,line width=0.03cm] (0,0) to (3,0);
                                \draw[->,line width=0.03cm] (0,0) to (0,3);

                                \draw[->,line width=0.03cm] (0,0) to (2.85,0.95);
                                \draw[->,line width=0.03cm] (0,0) to (-0.95,2.85);

                                \node[circle,fill,color=white] (a) at (0,0) {};

                                \node[circle,draw,line width=1pt] (a) at (0,0) {};
                                \node[circle,fill,inner sep=1pt] (b) at (0, 0) {};
        \end{tikzpicture} & \end{tabular}

    \begin{tabular}{cccccc}
        $\begin{bmatrix}A_{1} & 0 & 0\\0 & B_{1} & 0\\0 & 0 & B_{1}\end{bmatrix}$ & $\begin{bmatrix}A_{2} & 0 & - E_{2}\\0 & B_{2} & 0\\- E_{2} & 0 & C_{2}\end{bmatrix}$ & $\begin{bmatrix}A_{3} & 0 & 0\\0 & B_{3} & 0\\0 & 0 & B_{3}\end{bmatrix}$ & \end{tabular}

    \begin{align*}
        \overrightarrow{V_{G_2 \in 2/0}}&=- ((a \cdot \overrightarrow{z_{0}} + \lambda \cdot \overrightarrow{x_{2}}) \land \dot{\theta} \cdot \overrightarrow{z_{2}})\\
        &=\lambda \times \dot{\theta} \cdot \overrightarrow{y_{2}}\\
    \end{align*}

    \vspace{1em}
    \begin{align*}
        \overrightarrow{\Gamma_{G_2 \in 2/0}}&=\left.\dfrac{d \lambda \times \dot{\theta} \cdot \overrightarrow{y_{2}}}{dt}\right|_{R_{0}}\\
        &=(\lambda \times \ddot{\theta} \cdot \overrightarrow{y_{2}} + \lambda \times \dot{\theta} \cdot (\dot{\theta} \cdot \overrightarrow{z_{2}} \land \overrightarrow{y_{2}}))\\
        &=(\lambda \times \ddot{\theta} \cdot \overrightarrow{y_{2}} - \lambda \times \dot{\theta} \times \dot{\theta} \cdot \overrightarrow{x_{2}})\\
    \end{align*}

    \vspace{3em}
    \begin{align*}
        \overrightarrow{\sigma_{O \in 2/0}}&=( - E_{2} \times \dot{\theta} \cdot \overrightarrow{x_{2}} + C_{2} \times \dot{\theta} \cdot \overrightarrow{z_{2}} - ((a \cdot \overrightarrow{z_{0}} + \lambda \cdot \overrightarrow{x_{2}}) \land M_2 \cdot ((a \cdot \overrightarrow{z_{0}} + \lambda \cdot \overrightarrow{x_{2}}) \land \dot{\theta} \cdot \overrightarrow{z_{2}})))\\
        &=( - E_{2} \times \dot{\theta} \cdot \overrightarrow{x_{2}} + C_{2} \times \dot{\theta} \cdot \overrightarrow{z_{2}} - a \times M_2 \times \lambda \times \dot{\theta} \cdot \overrightarrow{x_{2}} + \lambda \times M_2 \times \lambda \times \dot{\theta} \cdot \overrightarrow{z_{2}})\\
    \end{align*}

    \vspace{3em}
    \begin{align*}
        \overrightarrow{\sigma_{G_2 \in 2/0}}&=( - E_{2} \times \dot{\theta} \cdot \overrightarrow{x_{2}} + C_{2} \times \dot{\theta} \cdot \overrightarrow{z_{2}})\\
    \end{align*}

    \vspace{1em}
    \begin{align*}
        \overrightarrow{\delta_{O \in 2/0}}&=(\left.\dfrac{d ( - E_{2} \times \dot{\theta} \cdot \overrightarrow{x_{2}} + C_{2} \times \dot{\theta} \cdot \overrightarrow{z_{2}})}{dt}\right|_{R_{0}} + ((a \cdot \overrightarrow{z_{0}} + \lambda \cdot \overrightarrow{x_{2}}) \land M_2 \cdot (\lambda \times \ddot{\theta} \cdot \overrightarrow{y_{2}} - \lambda \times \dot{\theta} \times \dot{\theta} \cdot \overrightarrow{x_{2}})))\\
        &=( - E_{2} \times \ddot{\theta} \cdot \overrightarrow{x_{2}} - E_{2} \times \dot{\theta} \cdot (\dot{\theta} \cdot \overrightarrow{z_{2}} \land \overrightarrow{x_{2}}) + C_{2} \times \ddot{\theta} \cdot \overrightarrow{z_{2}} + C_{2} \times \dot{\theta} \cdot (\dot{\theta} \cdot \overrightarrow{z_{2}} \land \overrightarrow{z_{2}}) + a \times M_2 \cdot ( - \lambda \times \ddot{\theta} \cdot \overrightarrow{x_{2}} - \lambda \times \dot{\theta} \times \dot{\theta} \cdot \overrightarrow{y_{2}}) + \lambda \times M_2 \times \lambda \times \ddot{\theta} \cdot \overrightarrow{z_{2}})\\
        &=( - E_{2} \times \ddot{\theta} \cdot \overrightarrow{x_{2}} - E_{2} \times \dot{\theta} \times \dot{\theta} \cdot \overrightarrow{y_{2}} + C_{2} \times \ddot{\theta} \cdot \overrightarrow{z_{2}} + a \times M_2 \cdot ( - \lambda \times \ddot{\theta} \cdot \overrightarrow{x_{2}} - \lambda \times \dot{\theta} \times \dot{\theta} \cdot \overrightarrow{y_{2}}) + \lambda \times M_2 \times \lambda \times \ddot{\theta} \cdot \overrightarrow{z_{2}})\\
    \end{align*}

\end{document}